\documentclass[a4paper,10pt,fleqn]{article}
\usepackage[margin=20mm]{geometry}
\usepackage{mathpazo,amsmath,amsfonts,amssymb}
\newcommand*{\md}[1]{\mathrm{d}#1}
\newcommand*{\sign}[1]{\mathrm{sign}\left(#1\right)}
\newcommand*{\pfrac}[2]{\dfrac{\partial#1}{\partial#2}}
\newcommand*{\ddfrac}[2]{\dfrac{\md#1}{\md#2}}
\title{Armstrong--Frederick Steel Model}
\author{Theodore Chang}
\date{}\pagestyle{empty}
\begin{document}
\noindent{}This document introduces the implementation of the uniaxial version of the Armstrong--Frederick Steel Model.
\section{Yield Function}
A von Mises yielding function is used.
\begin{gather}
F=\Big|\eta\Big|-k,
\end{gather}
in which $\eta=\sigma-\beta$ is the shifted stress, $\sigma$ is the stress, $\beta$ is the back stress and $k$ is the isotropic hardening stress.
\section{Flow Rule}
The associated plasticity flow is adopted. The plastic strain rate is then
\begin{gather}
\md{\varepsilon^p}=\gamma\pfrac{F}{\sigma}=\gamma{}n=\gamma~\sign{\eta},
\end{gather}
where $n=\dfrac{\eta}{\Big|\eta\Big|}=\sign{\eta}$. The corresponding accumulated plastic strain rate is
\begin{gather}
\md{p}=\Big|\md{\varepsilon^p}\Big|=\gamma.
\end{gather}
\section{Hardening Rules}
An exponential function with a linear component is used for isotropic hardening stress.
\begin{gather}
k=\sigma_y+k_lp+k_s-k_se^{-mp}.
\end{gather}
The corresponding derivative is
\begin{gather}
\ddfrac{k}{\gamma}=k_l+k_sme^{-mp}.
\end{gather}
The rate form of back stress $\displaystyle\beta=\sum\beta^i$ is defined as
\begin{gather*}
\md{\beta^i}=a^i\md{\varepsilon^p}-b^i\beta^i\md{p}.
\end{gather*}
In terms of $\gamma$, it is $\md{\beta^i}=a^i\gamma{}n-b^i\beta^i\gamma$. The incremental form is thus
\begin{gather}
\beta^i=\beta_n^i+a^i\gamma{}n-b^i\beta^i\gamma,\qquad
\beta^i=\dfrac{\beta_n^i+a^i\gamma{}n}{1+b^i\gamma}.
\end{gather}
\section{Incremental Form}
The shifted stress can be computed as
\begin{gather}
\eta=\sigma-\beta=E\left(\varepsilon^{tr}-\varepsilon^p_n-\gamma{}n\right)-\beta=\sigma^{tr}-nE\gamma-\sum\dfrac{\beta_n^i+na^i\gamma}{1+b^i\gamma}
\end{gather}
with $\sigma^{tr}=E(\varepsilon^{tr}-\varepsilon^p_n)$. Hence,
\begin{gather*}
\Big|\eta\Big|+E\gamma+\sum\dfrac{a^i\gamma}{1+b^i\gamma}=\Big|\sigma^{tr}-\sum\dfrac{\beta_n^i}{1+b^i\gamma}\Big|.
\end{gather*}
Eventually,
\begin{gather}
\Big|\eta\Big|=\Big|\sigma^{tr}-\sum\dfrac{\beta_n^i}{1+b^i\gamma}\Big|-E\gamma-\sum\dfrac{a^i\gamma}{1+b^i\gamma}.
\end{gather}
Then $\eta$ can be expressed as,
\begin{gather*}
\eta=\dfrac{\Big|\sigma^{tr}-\sum\dfrac{\beta_n^i}{1+b^i\gamma}\Big|-E\gamma-\sum\dfrac{a^i\gamma}{1+b^i\gamma}}{\Big|\sigma^{tr}-\sum\dfrac{\beta_n^i}{1+b^i\gamma}\Big|}\left(\sigma^{tr}-\sum\dfrac{\beta_n^i}{1+b^i\gamma}\right).
\end{gather*}
It is equivalent to
\begin{gather*}
\eta=\left(\Big|\sigma^{tr}-\sum\dfrac{\beta_n^i}{1+b^i\gamma}\Big|-E\gamma-\sum\dfrac{a^i\gamma}{1+b^i\gamma}\right)u.
\end{gather*}
It is easy to see that $n=u$ with $\displaystyle{}u=\dfrac{\sigma^{tr}-\sum\dfrac{\beta_n^i}{1+b^i\gamma}}{\Big|\sigma^{tr}-\sum\dfrac{\beta_n^i}{1+b^i\gamma}\Big|}$.
\section{Scalar Equation Iteration}
The yield function is then
\begin{gather}
F=\Big|\sigma^{tr}-\sum\dfrac{\beta_n^i}{1+b^i\gamma}\Big|-E\gamma-\sum\dfrac{a^i\gamma}{1+b^i\gamma}-\left(\sigma_y+k_l\left(p_n+\gamma\right)+k_s\left(1-e^{-m\left(p_n+\gamma\right)}\right)\right).
\end{gather}
The corresponding derivative is then
\begin{gather}
\pfrac{F}{\gamma}=\sum\dfrac{b^i\beta_n^iu-a^i}{(1+b^i\gamma)^2}-E-k_l-k_sme^{-m\left(p_n+\gamma\right)},\qquad
\pfrac{F}{\varepsilon^{tr}}=Eu.
\end{gather}
\section{Consistent Tangent Stiffness}
For stiffness, $\varepsilon^{tr}$ is now varying, then
\begin{gather}
\pfrac{F}{\varepsilon^{tr}}+\pfrac{F}{\gamma}\ddfrac{\gamma}{\varepsilon^{tr}}=0,\qquad\ddfrac{\gamma}{\varepsilon^{tr}}=-\left(\pfrac{F}{\gamma}\right)^{-1}\pfrac{F}{\varepsilon^{tr}}.
\end{gather}
Since the stress can be written as
\begin{gather}
\sigma=E(\varepsilon^{tr}-\varepsilon^p)=E(\varepsilon^{tr}-\varepsilon^p_n-\Delta\varepsilon^p)=E(\varepsilon^{tr}-\varepsilon^p_n)-E\gamma{}u.
\end{gather}
The derivative is
\begin{gather}
\ddfrac{\sigma}{\varepsilon^{tr}}=E-Eu\ddfrac{\gamma}{\varepsilon^{tr}}=E+E^2\left(\pfrac{F}{\gamma}\right)^{-1}.
\end{gather}
\end{document}
